systems/ChordSemantics.v
@@ -1,0 +1,123 @@
+Require Import Chord.Chord.
+Require Import Chord.ChordLocalProps.
+Require Import Verdi.DynamicNet.
+Require Import List.
+
+Module ConstrainedChord <: ConstrainedDynamicSystem.
+  Include Chord.
+
+  Definition msg : Type := (addr * (addr * payload))%type.
+
+  Inductive event : Type :=
+  | e_send : msg -> event
+  | e_recv : msg -> event
+  | e_timeout : addr -> timeout -> event
+  | e_fail : addr -> event.
+
+  Record global_state :=
+    { nodes : list addr;
+      failed_nodes : list addr;
+      timeouts : addr -> list timeout;
+      sigma : addr -> option data;
+      msgs : list msg;
+      trace : list event
+    }.
+
+  Inductive timeout_constraint_ : global_state -> addr -> timeout -> Prop :=
+  | Tick_unconstrained : forall gst h,
+      timeout_constraint_ gst h Tick
+  | KeepaliveTick_unconstrained : forall gst h,
+      timeout_constraint_ gst h KeepaliveTick
+  | Request_needs_dst_dead_and_no_msgs : forall gst dst h p,
+      In dst (failed_nodes gst) ->
+      (forall m, request_response_pair p m -> ~ In (dst, (h, m)) (msgs gst)) ->
+      timeout_constraint_ gst h (Request dst p).
+  Definition timeout_constraint := timeout_constraint_.
+
+  Definition timeouts_detect_failure (gst : global_state) : Prop :=
+    forall xs t ys h dead req,
+      (trace gst) = xs ++ t :: ys ->
+      (* if a request timeout occurs at some point in the trace... *)
+      t = (e_timeout h (Request dead req)) ->
+      (* then it corresponds to an earlier node failure. *)
+      In (e_fail dead) xs.
+
+  (* tip: treat this as opaque and use lemmas: it never gets stopped except by failure *)
+  Definition live_node (gst : global_state) (h : addr) : Prop :=
+    In h (nodes gst) /\
+    ~ In h (failed_nodes gst) /\
+    exists st,
+      sigma gst h = Some st /\
+      joined st = true.
+
+  Definition dead_node (gst : global_state) (h : addr) : Prop :=
+    In h (nodes gst) /\
+    In h (failed_nodes gst) /\
+    exists st,
+      sigma gst h = Some st.
+
+  Definition joining_node (gst : global_state) (h : addr) : Prop :=
+    exists st,
+      sigma gst h = Some st /\
+      joined st = false /\
+      In h (nodes gst) /\
+      ~ In h (failed_nodes gst).
+
+  Definition best_succ (gst : global_state) (h s : addr) : Prop :=
+    exists st xs ys,
+      live_node gst h /\
+      sigma gst h = Some st /\
+      map addr_of (succ_list st) = xs ++ s :: ys /\
+      (forall o, In o xs -> dead_node gst o) /\
+      live_node gst s.
+
+  Definition live_node_in_succ_lists (gst : global_state) : Prop :=
+    forall h st,
+      sigma gst h = Some st ->
+      live_node gst h ->
+      exists s,
+        best_succ gst h s.
+
+  (* This is a way of dealing with succ lists missing entries
+     mid-stabilization that doesn't involve putting artificial entries
+     into the actual successor list. *)
+  Definition ext_succ_list_span_includes (h : id) (succs : list id) (n : id) :=
+    forall n l e,
+      length (h :: succs) = n ->
+      l = last succs h ->
+      e = l + (Chord.SUCC_LIST_LEN - n) ->
+      between h n e.
+
+  (* "A principal node is a member that is not skipped by any member's
+     extended successor list" *)
+  Definition principal (gst : global_state) (p : addr) : Prop :=
+    forall h st succs,
+      live_node gst h ->
+      sigma gst h = Some st ->
+      map id_of (succ_list st) = succs ->
+      ext_succ_list_span_includes h succs p ->
+      In p succs.
+
+  Definition principals (gst : global_state) (ps : list addr) : Prop :=
+    NoDup ps /\
+    Forall (principal gst) ps /\
+    forall p, principal gst p -> In p ps.
+
+  Definition sufficient_principals (gst : global_state) : Prop :=
+    exists ps,
+      principals gst ps /\
+      length ps > Chord.SUCC_LIST_LEN.
+
+  Definition principal_failure_constraint (gst : global_state) (f : addr) : Prop :=
+    principal gst f ->
+    forall ps,
+      principals gst ps ->
+      length ps > (Chord.SUCC_LIST_LEN + 1).
+
+  Definition failure_constraint (gst : global_state) (f : addr) (gst' : global_state) : Prop :=
+    live_node_in_succ_lists gst' /\
+    principal_failure_constraint gst f.
+
+End ConstrainedChord.
+
+Module ChordSemantics := DynamicSemantics(ConstrainedChord).
